Split main result.

theories/Sorting.v
@@ -15,12 +15,25 @@ Section Sorting.
 
 (** In this post, we will formalize one of the most well-known results
 of algorithm analysis: no comparison sort can run in less than [O(n *
-log n)] steps when sorting an array of size [n].
+log n)] steps on an array of size [n].
 
-First, we must define a convenient datatype for representing the
-execution of a sorting algorithm. For our purposes, a sorting
-algorithm can be seen as a binary tree: internal nodes denote a
-comparison between two elements, with the right and left branches
+Before starting, I should point out that this is the first post in
+this blog to use the Ssreflect and the Mathematical Components #<a
+href="http://ssr.msr-inria.inria.fr">libraries</a>#. Ssreflect is an
+amazing Coq extension that brings several improvements, including a
+nicer set of base tactics. Both libraries cover a wide range of
+theories, including fairly sophisticated Mathematics - as a matter of
+fact, both libraries form the basis of the Coq formalization of the
+#<a
+href="http://en.wikipedia.org/wiki/Feit%E2%80%93Thompson_theorem">Feit-Thompson
+theorem</a>#, known for its extremely complex and detailed proof. The
+theory of permutations over finite types available in the Mathematical
+Components library will be particularly useful for our problem.
+
+We'll begin our formalization by defining a convenient datatype for
+representing the execution of a sorting algorithm. For our purposes, a
+sorting algorithm can be seen as a binary tree: internal nodes denote
+a comparison between two elements, with the right and left branches
 telling how to proceed on each case. The leaves of the tree signal
 that the algorithm halted, producing a result. This results in the
 following type: *)
@@ -31,14 +44,13 @@ Inductive sort_alg (n : nat) : Type :=
 
 (** Let's analyze this declaration in detail. The [n] parameter will
 be used later to track the length of the array that we are
-sorting. ['I_n] and ['S_n] are types defined in Ssreflect: the former
-is the type of natural numbers bounded by [n], whereas the latter
-represents permutations of that type. The idea is that, when running
-our algorithm, the [i] and [j] arguments of [Compare] tell which
-elements of our array to compare. The permutation in [Done] specifies
-how to rearrange the elements of the input array to produce an
-answer. We can formalize the previous description in the following
-function: *)
+sorting. ['I_n] is the type of natural numbers bounded by [n], whereas
+['S_n] represents permutations of elements of that type. The idea is
+that, when running our algorithm, the [i] and [j] arguments of
+[Compare] tell which elements of our array to compare. The permutation
+in [Done] specifies how to rearrange the elements of the input array
+to produce an answer. We can formalize the previous description in the
+following function: *)
 
 Fixpoint execute T n c (a : sort_alg n) (xs : n.-tuple T) :=
   match a with
@@ -57,27 +69,89 @@ how to rearrange [a]'s elements.
 With [execute], we can now define what it means for a sorting
 algorithm to be correct: *)
 
-Definition sort_alg_ok (a : forall n, sort_alg n) :=
+Definition sort_alg_ok n (a : sort_alg n) :=
   forall (T : eqType) (le : rel T),
-  forall n xs, execute le (a n) xs = sort le xs :> seq T.
+  forall xs, execute le a xs = sort le xs :> seq T.
 
 (** With [sort_alg_ok] in hand, we are ready to formulate our main
-result. Informally, our proof works as follows:
+result. Informally, its proof works as follows:
 
   - In the worst case, an array of size [n] has [n!] permutations.
 
   - A sorting algorithm can distinguish at most [2 ^ k] permutations,
     where [k] is the maximum number of comparisons performed.
 
-  - Therefore, [n! <= 2 ^ k], implying [log_2 n! <= k].
+  - Since our algorithm must work on every possible permutation of a
+    given array, we know that [n! <= 2 ^ k]. By taking the logarithm
+    of both sides, we get [log2 n! <= k].
 
-  - Using Stirling's approximation, we can weaken this lower bound and
-    derive the final result.
+  - Stirling's approximation tells us that the left-hand side of this
+    inequality grows like [n * log n], modulo a multiplicative
+    constant. This allows us to conclude.
 
-Unfortunately, we don't have a Coq proof of Stirling's approximation
-we can use here, which forces us to adapt the last step. We show the
-following lemma by induction ([trunc_log], as its name says, is the
-truncated logarithm): *)
+Using the Mathematical Components library, we can formalize almost all
+of the above steps. For instance, here's how we bound the number of
+permutations an algorithm can distinguish: *)
+
+Fixpoint comparisons n (a : sort_alg n) : nat :=
+  match a with
+  | Compare _ _ l r => (maxn (comparisons l) (comparisons r)).+1
+  | Done _ => 0
+  end.
+
+Fixpoint perms n (a : sort_alg n) : {set 'S_n} :=
+  match a with
+  | Compare _ _ l r => perms l :|: perms r
+  | Done p => [set p]
+  end.
+
+Lemma card_perms n (a : sort_alg n) : #|perms a| <= 2 ^ comparisons a.
+Proof.
+elim: a=> [i j l IHl r IHr|p] /=; last by rewrite cards1.
+rewrite (leq_trans (leq_of_leqif (leq_card_setU (perms l) (perms r)))) //.
+by rewrite expnS mul2n -addnn leq_add // ?(leq_trans IHl, leq_trans IHr) //
+   leq_exp2l // ?(leq_maxl, leq_maxr).
+Qed.
+
+(** A crucial part of the above argument, that was left implicit, was
+showing that a correct comparison sort must contain all possible
+permutations: *)
+
+(* begin hide *)
+Section WithGroupScope.
+Import GroupScope.
+(* end hide *)
+Lemma permsT n (a : sort_alg n) : sort_alg_ok a -> perms a = [set: 'S_n].
+Proof.
+move=> a_ok.
+apply/eqP; rewrite -subTset; apply/subsetP=> /= p _.
+move: {a_ok} (a_ok _ leq [tuple val (p^-1 i) | i < n]).
+rewrite (_ : sort _ _ = [tuple val i | i < n]); last first.
+  apply: (eq_sorted leq_trans anti_leq (sort_sorted leq_total _)).
+    by rewrite /= val_enum_ord iota_sorted.
+  rewrite (perm_eq_trans (introT perm_eqlP (perm_sort _ _))) //.
+  apply/tuple_perm_eqP; exists p^-1; congr val; apply/eq_from_tnth=> i.
+  by rewrite 3!tnth_map 2!tnth_ord_tuple.
+elim: a=> [/= i j l IHl r IHr|p'].
+  by case: ifP=> [_ /IHl|_ /IHr]; rewrite in_setU => -> //; rewrite orbT.
+move/val_inj=> /=.
+rewrite in_set1=> e; apply/eqP/permP=> i; apply/esym/(canRL (permKV p)).
+apply/val_inj.
+rewrite (_ : val i = tnth [tuple val i | i < n] i); last first.
+  by rewrite tnth_map tnth_ord_tuple.
+by rewrite -{}e 2!tnth_map !tnth_ord_tuple.
+Qed.
+(* begin hide *)
+End WithGroupScope.
+(* end hide *)
+
+(** Notice how we leveraged the finite sets of Mathematical Components
+to help us here.
+
+Unfortunately, we don't have a proof of Stirling's approximation we
+can use for the last step, which forces us to take a more direct
+route. We show the following lemma by induction ([trunc_log], as its
+name says, is the truncated logarithm): *)
 
 Local Notation log2 := (trunc_log 2).
 
@@ -85,9 +159,7 @@ Lemma log2_fact n : (n * log2 n)./2 <= log2 n`!.
 Proof.
 (** In order to get our proof to go through, we must strengthen our
 induction hypothesis a little bit: *)
-
 suff: n * (log2 n).+2 <= (log2 n`! + 2 ^ (log2 n)).*2.+1.
-  (* ... *)
   (* begin hide *)
   move: (leq0n n); rewrite leq_eqVlt=> /orP [/eqP <- //|pos].
   move/half_leq; rewrite -(addn1 _.*2) halfD odd_double add0n addn0 doubleK.
@@ -95,15 +167,13 @@ suff: n * (log2 n).+2 <= (log2 n`! + 2 ^ (log2 n)).*2.+1.
   rewrite (addnC (log2 _)) -leq_subLR -addnBA ?trunc_logP //.
   exact/leq_trans/leq_addr.
   (* end hide *)
-have [|] := boolP (3 <= n); last by case: n => [|[|[|[|]]]] //=.
+(** We can then proceed with a reasonably straightforward inductive
+argument. *)
 elim: n=> [|n IH] //=.
-rewrite leq_eqVlt=> /orP [/eqP <- //|lb]; move/(_ lb) in IH.
-
-(** On the inductive step, we also have two cases to consider: whether
-or not [log2 n] is less than [log2(n.+1)]. *)
-have: log2 n.+1 = log2 n \/ log2 n.+1 = (log2 n).+1 /\ 2 ^ (log2 n.+1) = n.+1.
 (* ... *)
 (* begin hide *)
+have [lb|] := boolP (3 <= n); last by case: n IH => [|[|[|[|]]]] //=.
+have: log2 n.+1 = log2 n \/ log2 n.+1 = (log2 n).+1 /\ 2 ^ (log2 n.+1) = n.+1.
   move: (@trunc_log_bounds 2 _ erefl (@leq_trans 3 1 n erefl lb))
         (@trunc_log_bounds 2 _ erefl (@leq_trans 4 1 n.+1 erefl lb))
         => /andP [e1 e2] /andP [e3 e4].
@@ -131,49 +201,18 @@ by rewrite -addnn leq_add2l.
 (* end hide *)
 Qed.
 
-Fixpoint comparisons n (a : sort_alg n) : nat :=
-  match a with
-  | Compare _ _ l r => (maxn (comparisons l) (comparisons r)).+1
-  | Done _ => 0
-  end.
-
 (* begin hide *)
 Import GroupScope.
 (* end hide *)
-Lemma sort_alg_ok_leq n a :
-  sort_alg_ok a -> (n * log2 n)./2 <= comparisons (a n).
+(** We can now conclude with our main result: *)
+Lemma sort_alg_ok_leq n (a : sort_alg n) :
+  sort_alg_ok a -> (n * log2 n)./2 <= comparisons a.
 Proof.
-move/(_ _ _ n); move: {a} (a n) => a a_ok.
-suff lb: n`! <= 2 ^ comparisons a.
+move=> a_ok; suff lb: n`! <= 2 ^ comparisons a.
   rewrite (leq_trans (log2_fact n)) // -(@leq_exp2l 2) //.
   by rewrite (leq_trans (trunc_logP (leqnn 2) (fact_gt0 n))).
-pose fix ps a : {set 'S_n} :=
-  match a with
-  | Compare _ _ l r => ps l :|: ps r
-  | Done p => [set p]
-  end.
-have ub: #|ps a| <= 2 ^ comparisons a.
-  elim: {a_ok} a=> [i j l IHl r IHr|p] /=; last by rewrite cards1.
-  rewrite (leq_trans (leq_of_leqif (leq_card_setU (ps l) (ps r)))) //.
-  by rewrite expnS mul2n -addnn leq_add // ?(leq_trans IHl, leq_trans IHr) //
-     leq_exp2l // ?(leq_maxl, leq_maxr).
-rewrite (leq_trans _ ub) // {ub} -{1}(card_ord n) -cardsT -card_perm.
-rewrite -(cardsE (perm_on [set: 'I_n])) subset_leq_card //.
-apply/subsetP=> /= p _; move: {a_ok} (a_ok _ leq [tuple val (p^-1 i) | i < n]).
-rewrite (_ : sort _ _ = [tuple val i | i < n]); last first.
-  apply: (eq_sorted leq_trans anti_leq (sort_sorted leq_total _)).
-    by rewrite /= val_enum_ord iota_sorted.
-  rewrite (perm_eq_trans (introT perm_eqlP (perm_sort _ _))) //.
-  apply/tuple_perm_eqP; exists p^-1; congr val; apply/eq_from_tnth=> i.
-  by rewrite 3!tnth_map 2!tnth_ord_tuple.
-elim: a=> [/= i j l IHl r IHr|p'].
-  by case: ifP=> [_ /IHl|_ /IHr]; rewrite in_setU => -> //; rewrite orbT.
-move/val_inj=> /= {ps}.
-rewrite in_set1=> e; apply/eqP/permP=> i; apply/esym/(canRL (permKV p)).
-apply/val_inj.
-rewrite (_ : val i = tnth [tuple val i | i < n] i); last first.
-  by rewrite tnth_map tnth_ord_tuple.
-by rewrite -{}e 2!tnth_map !tnth_ord_tuple.
+rewrite (leq_trans _ (card_perms a)) // -{1}(card_ord n) -cardsT -card_perm.
+by rewrite -(cardsE (perm_on [set: 'I_n])) subset_leq_card // permsT //.
 Qed.
 
 (* begin hide *)
